frodo/spec/Spec.Frodo.Sample.fst
@@ -16,32 +16,58 @@ module Matrix = Spec.Matrix
 
 let cdf_table_len = size_v cdf_table_len
 
-let cdf_table: lseq uint16 cdf_table_len = 
+let cdf_table: lseq uint16 cdf_table_len =
   assert_norm (List.Tot.length cdf_list == cdf_table_len);
   Seq.createL cdf_list
 
-val frodo_sample: r:uint16 -> uint16
-let frodo_sample r =
+val frodo_sample_f:
+    t:uint16
+  -> i:size_nat{i < cdf_table_len}
+  -> res:nat{res = 0 \/ res = 1}
+let frodo_sample_f t i =
   let open Lib.RawIntTypes in
-  let t = r >>. u32 1 in
-  let r0 = r &. u16 1 in
-  mod_mask_lemma r (u32 1);
-  uintv_extensionality (mod_mask (u32 1)) (u16 1);
-  assert (uint_v r0 == 0 \/ uint_v r0 == 1);
-  let e = 0 in
-  let e =
-    repeati_inductive
-      (cdf_table_len - 1)
-      (fun z e -> 0 <= e /\ e <= z /\ z < cdf_table_len)
-      (fun z e -> let e = if (uint_to_nat t > uint_to_nat cdf_table.[z]) then e + 1 else e in e)
-      e
-  in
+  if (uint_to_nat t > uint_to_nat cdf_table.[i])
+  then 1 else 0
+
+val frodo_sample_fc:
+    t:uint16
+  -> i:size_nat{i <= cdf_table_len}
+  -> GTot (res:nat{0 <= res /\ res <= i})
+    (decreases i)
+let rec frodo_sample_fc t i =
+  if i = 0 then 0
+  else frodo_sample_f t (i - 1) + frodo_sample_fc t (i - 1)
+
+val frodo_sample_res:
+    r0:uint16{uint_v r0 == 0 \/ uint_v r0 == 1}
+  -> e:nat{e < cdf_table_len}
+  -> res:uint16
+let frodo_sample_res r0 e =
+  let open Lib.RawIntTypes in
   let open FStar.Math.Lib in
   let e = (powx (-1) (uint_to_nat r0)) * e in
   assert_norm (powx (-1) 1 == -1);
   assert_norm (powx (-1) 0 == 1);
   assert (-cdf_table_len < e /\ e < cdf_table_len);
   u16 (e % modulus U16)
+
+#set-options "--max_fuel 1"
+
+val frodo_sample: r:uint16 -> uint16
+let frodo_sample r =
+  let t = r >>. u32 1 in
+  let r0 = r &. u16 1 in
+  mod_mask_lemma r (u32 1);
+  uintv_extensionality (mod_mask (u32 1)) (u16 1);
+  assert (uint_v r0 == 0 \/ uint_v r0 == 1);
+  let e =
+    repeati_inductive
+      (cdf_table_len - 1)
+      (fun z e -> 0 <= e /\ e <= z /\ z < cdf_table_len /\ e == frodo_sample_fc t z)
+      (fun z e -> frodo_sample_f t z + e) 0 in
+  frodo_sample_res r0 e
+
+#set-options "--max_fuel 0"
 
 val frodo_sample_matrix_fc:
     n1:size_nat
